\documentclass[10pt, a4paper, nofootinbib]{scrartcl}

\newcommand{\pagetitle}{LMAT1271 : Project report} 

\input{../header}
\input{../preamble-exercice}

\pagenumbering{arabic}

\begin{document}

\section{Point estimation}

\subsection*{Context}
Our engineering team just landed a consulting contract with a company interested in the electricity consumption of its machines. In a first part, we would like to determine how electricity consumption is evenly distributed across the different machines of the same type. To this end, we use the Gini coefficient. In a nutshell, it is an index ranging from $0$ to $1$ measuring the inequality featured in a distribution. A value of $0$ denotes that all our machines use the same amount of electricity while a value of $1$ means that all the electricity is used by a single machine.
We assume that all of the $n$ machines operate independently and their daily electricity consumption (in MWh) can be modelled as a random variable $X$ with the following density function,

\begin{equation}
  f_{\theta_1, \theta_2}(x) = 
  \begin{cases}
    \frac{\theta_1 \theta_2^{\theta_1}}{x^{\theta_1 + 1}}, &\quad x \geq \theta_2 \\
    0,                                                     &\quad \text{otherwise}
  \end{cases}
\end{equation}

with $\theta_1 > 2$ and $\theta_2 > 0$.

\textbf{(a)} Derive the quantile function of $X$

\begin{center}\rule{6cm}{0.4pt}\end{center}

We're looking to solve $P(X \leq x_t) = t$ for $x_t$.

First let's compute $P(X \leq x_t)$, 
\begin{align*}
  P(X \leq x_t)
    &= \int_{-\infty}^{x_t} f_{\theta_1, \theta_2}(x) dx \\
    &= \int_{\theta_2}^{x_t} \theta_1 \theta_2^{\theta_1} x^{-(\theta_1 + 1)} dx \\
    &= - \frac{\theta_1 \theta_2^{\theta_1}}{\theta_1} \left[ x^{-\theta_1} \right]_{x=\theta_2}^{x=x_t} \\
    &= - \frac{\theta_1 \theta_2^{\theta_1}}{\theta_1} \left( x_t^{-\theta_1} - \theta_2^{-\theta_1} \right) \\
\end{align*}

Let's solve $P(X \leq x_t) = t$ for $x_t$,
\begin{align*}
  - \frac{\theta_1 \theta_2^{\theta_1}}{\theta_1} \left( x_t^{-\theta_1} - \theta_2^{-\theta_1} \right) = t 
    &\iff x_t^{\theta_1} 
      = \frac{t \theta_1}{\theta_1 \theta_2^{\theta_1}} - \theta_2^{-\theta_1} \\
    &\iff x_t 
      = \left( \frac{t \theta_1}{\theta_1 \theta_2^{\theta_1}} - \theta_2^{-\theta_1} \right)^{1/\theta_1} \equiv Q_{\theta_1, \theta_2}(t)
\end{align*}

\textbf{(b)} Derive the Gini coefficient of $X$.

\begin{center}\rule{6cm}{0.4pt}\end{center}

The Gini coefficient is defined as, 
\begin{equation}
  G_{\theta_1, \theta_2}(t) = 2 \int_{0}^{1} \left( p - \frac{\int_{0}^{p} Q(t) dt}{E(X)} \right) dp
\end{equation}

Let's first compute the mean of $X$,
\begin{align*}
  E(X)
    &= \int_{-\infty}^{+\infty} x f(x) dx \\
    &= \int_{\theta_2}^{+\infty} x \frac{\theta_1 \theta_2^{\theta_1}}{x^{\theta_1 + 1}} dx \\
    &= \theta_1 \theta_2^{\theta_1} \int_{\theta_2}^{+\infty} x^{- \theta_1} dx \\
    &= - \frac{\theta_1 \theta_2^{\theta_1}}{(\theta_1 - 1)} \left[ x^{-(\theta_1 - 1)} \right]_{\theta_2}^{+\infty}
\end{align*}

Then the Gini coefficient, 
\begin{align*}
  G_{\theta_1, \theta_2}
    &= 2 \left( \int_{0}^{1} p dp - \int_{0}^{1} \frac{\int_{0}^{p} Q(t) dt}{E(X)} dp \right) 
\end{align*}

We compute each integral separately,
\begin{align*}
  \int_0^p Q(t) dt 
    &= \int_0^p \left( \frac{t \theta_1}{\theta_1 \theta_2^{\theta_1}} - \theta_2^{-\theta_1} \right)^{1/\theta_1} dt
\end{align*}

We use the change of variable $u = \frac{t \theta_1}{\theta_1 \theta_2^{\theta_1}} - \theta_2^{-\theta_1}$, $du = \frac{\theta_1}{\theta_1 \theta_2^{\theta_1}} dt$

The boundaries becomes, 
\begin{align*}
  \begin{cases}
    t = 0 &\implies u_1 \equiv - \theta_2^{-\theta_1} \\
    t = p &\implies u_2 \equiv \frac{p \theta_1}{\theta_1 \theta_2^{\theta_1}} - \theta_2^{-\theta_1}
  \end{cases}
\end{align*}

Then, 
\begin{align*}
  \int_0^p Q(t) dt 
    &= \int_{u_1}^{u_2} u^{(1/\theta_1)} \frac{\theta_1 \theta_2^{\theta_1}}{\theta_1} du \\
    &= \frac{\theta_1}{\theta_1 \theta_2^{\theta_1}} \left[ \frac{u^{(1/\theta_1) + 1}}{(1/\theta_1) + 1} \right]_{u_1}^{u_2} \\
    &= \frac{\theta_1}{\theta_1 \theta_2^{\theta_1} ((1/\theta_1) + 1)} \left( \left( \frac{p \theta_1}{\theta_1 \theta_2^{\theta_1}} - \theta_2^{-\theta_1} \right)^{(1/\theta_1) + 1} - \left( - \theta_2^{-\theta_1} \right)^{(1/\theta_1) + 1} \right)
\end{align*}

Therefore, 
\begin{align*}
  \frac{\int_{0}^{p} Q(t) dt}{E(X)}
    &= \frac{\theta_1(\theta_1 - 1)}{\theta_2^{(1 - \theta_1)} ((1/\theta_1) + 1)} \left( \left( \frac{p \theta_1}{\theta_1 \theta_2^{\theta_1}} - \theta_2^{-\theta_1} \right)^{(1/\theta_1) + 1} - \left( - \theta_2^{-\theta_1} \right)^{(1/\theta_1) + 1} \right)
\end{align*}

Then,
\begin{align*}
  \int_{0}^{1} \frac{\int_{0}^{p} Q(t) dt}{E(X)} dp 
    &= \frac{\theta_1(\theta_1 - 1)}{\theta_2^{1 - \theta_1}} \left( \underbrace{\int_0^1 \left( \frac{p \theta_1}{\theta_1 \theta_2^{\theta_1}} - \theta_2^{-\theta_1} \right)^{(1/\theta_1) + 1} dp}_{\equiv A} - \underbrace{\int_0^1 \left( - \theta_2^{-\theta_1} \right)^{(1/\theta_1) + 1} dp}_{\equiv B} \right)
\end{align*}

Computing integral A and B. For A we use the same change of variable as before,
\begin{align*}
  A 
    &= \int_{u_1}^{u_2} u^{(1/\theta_1) + 1} \frac{\theta_1 \theta_2^{\theta_1}}{\theta_1} du \\
    &= \frac{\theta_1 \theta_2^{\theta_1}}{\theta_1} \left( \left( \frac{\theta_1}{\theta_1 \theta_2^{\theta_1}} - \theta_2^{-\theta_1} \right)^{(1/\theta_1) + 2} - \left( - \theta_2^{-\theta_1} \right)^{(1/\theta_1) + 2} \right)
\end{align*}

\begin{align*}
  B 
    &= \left( - \theta_2^{-\theta_1} \right)^{(1/\theta_1) + 1} \int_0^1 dp \\
    &= \left( - \theta_2^{-\theta_1} \right)^{(1/\theta_1) + 1}
\end{align*}

Then, 
\begin{align*}
  \int_0^1 pdp 
    &= \frac{1}{2}
\end{align*}

Eventually,
\begin{align*}
  G_{\theta_1, \theta_2} 
    &= 2 \left( \frac{1}{2} - \frac{\theta_1(\theta_1 - 1)}{\theta_2^{(1 - \theta_1)} ((1/\theta_1) + 1)} \left[ \frac{\theta_1 \theta_2^{\theta_1}}{\theta_1} \frac{1}{(1/\theta_1) + 2} \left( \left( \frac{\theta_1}{\theta_1 \theta_2^{\theta_1}} - \theta_2^{-\theta_1} \right)^{(1/\theta_1) + 2} - \left( - \theta_2^{-\theta_1} \right)^{(1/\theta_1) + 2} \right) \\
    & - \left( - \theta_2^{-\theta_1} \right)^{(1/\theta_1) + 1} \right] \right) 
\end{align*}

\end{document}
